devel/Iron/Language/SimpleDelayed/Exp.v
@@ -3,13 +3,20 @@ Require Export Iron.Language.SimpleDelayed.Base.
 Require Export Iron.Language.SimpleDelayed.Ty.
 
 
+
 (* Value Expressions *)
 Inductive exp : Type :=
- | XVar    : nat       -> exp                        (* named variable. *)
- | XLam    : list bind -> nat -> ty  -> exp -> exp   (* function abstraction *)
- | XApp    : exp       -> exp -> exp                 (* function application *)
+ (* a named variable. *)
+ | XVar    : nat       -> exp
+
+ (* function abstraction *)
+ | XAbs    : list bind -> nat -> ty  -> exp -> exp   
+
+ (* function application *)
+ | XApp    : exp       -> exp -> exp
 
 with bind  : Type := 
+ (* binding in a substitution. *)
  | BBind   : nat -> ty -> exp -> bind.
 
 Hint Constructors exp.
@@ -20,19 +27,20 @@ Hint Constructors bind.
 Definition substx := list bind.
 
 
+(********************************************************************)
 (* Mutual induction principle for expressions. *)
 Theorem exp_mutind
  : forall
     (PX  : exp        -> Prop)
     (PB  : bind       -> Prop)
  ,  (forall n,                                  PX (XVar n))
- -> (forall bs n t x, Forall PB bs -> PX x   -> PX (XLam bs n t x))
+ -> (forall bs n t x, Forall PB bs -> PX x   -> PX (XAbs bs n t x))
  -> (forall x1 x2,    PX x1  -> PX x2        -> PX (XApp x1 x2))
  -> (forall n t x,    PX x                   -> PB (BBind  n t x))
  -> forall x, PX x.
 Proof.
  intros PX PB.
- intros var lam app bind.
+ intros var abs app bind.
  refine (fix   IHX x : PX x := _  
          with  IHB b : PB b := _ 
          for  IHX).
@@ -40,7 +48,7 @@ Proof.
  - Case "expressions".
    case x; intros.
    + apply var.
-   + apply lam. induction l; intuition. apply IHX.
+   + apply abs. induction l; intuition. apply IHX.
    + apply app. apply IHX. apply IHX.
 
  - Case "bindings".
@@ -49,40 +57,84 @@ Proof.
 Qed.
 
 
-Definition isXLam (x1: exp): Prop := 
- (exists bs n t x, x1 = XLam bs n t x).
+(********************************************************************)
+(* Predicates. *)
+Definition isXAbs (x1: exp): Prop := 
+ (exists bs n t x, x1 = XAbs bs n t x).
 
 
-Lemma isXLam_true
- : forall bs n t x, isXLam (XLam bs n t x).
+Lemma isXAbs_true
+ : forall bs n t x, isXAbs (XAbs bs n t x).
 Proof.
  intros.
- unfold isXLam.
+ unfold isXAbs.
  exists bs. exists n. exists t. exists x.
  trivial.
 Qed.
-Hint Resolve isXLam_true.
+Hint Resolve isXAbs_true.
 
 
-Lemma isXLam_XVar
+Lemma isXAbs_XVar
  : forall n
- , ~isXLam (XVar n).
-Proof. 
- intuition.
- firstorder.
- congruence.
-Qed.
-Hint Resolve isXLam_XVar.
-
-
-Lemma isXLam_XApp
- : forall x1 x2
- , ~isXLam (XApp x1 x2).
+ , ~isXAbs (XVar n).
 Proof.
- intuition.
- firstorder.
- congruence.
+ intuition. nope.
 Qed.
-Hint Resolve isXLam_XApp.
+Hint Resolve isXAbs_XVar.
 
+
+Lemma isXAbs_XApp
+ : forall x1 x2
+ , ~isXAbs (XApp x1 x2).
+Proof.
+ intuition. nope.
+Qed.
+Hint Resolve isXAbs_XApp.
+
+
+(********************************************************************)
+(* Values *)
+Inductive Value : exp -> Prop :=
+ | ValueAbs 
+   :  forall bs v t x
+   ,  Value (XAbs bs v t x).
+
+Hint Constructors Value.
+
+
+Lemma isValue_not_var
+ : forall n
+ , ~Value (XVar n).
+Proof.
+ intros. intuition. inverts H.
+Qed.
+Hint Resolve isValue_not_var.
+
+
+Lemma isValue_not_app
+ : forall x1 x2
+ , ~Value (XApp x1 x2).
+Proof.
+ intros. intuition. inverts H.
+Qed.
+Hint Resolve isValue_not_app.
+
+
+(* Done expressions have finished evaluating. *)
+Inductive Done  : exp -> Prop :=
+ | DoneVar 
+   :  forall n
+   ,  Done (XVar n)
+
+ | DoneValue
+   :  forall x
+   ,  Value  x
+   -> Done   x
+
+ | DoneApp 
+   :  forall x1 x2
+   ,  Done x1 /\ ~Value x1
+   -> Done (XApp x1 x2).
+
+Hint Constructors Done.
 
