devel/Iron/Language/SimpleDelayed/Ty.v
@@ -20,9 +20,11 @@ Definition tyenv := list sig.
 (* Lookup the type of the given variable from the environment. *)
 Fixpoint lookupEnv (var: nat) (te: tyenv) : option ty :=
  match te with
- | nil                => None
+ | nil                
+ => None
+
  | SSig v t :: rest
-    => if beq_nat var v
+ => if beq_nat var v
         then Some t
         else lookupEnv var rest
  end.
