done/Iron/Data/List/Forall.v
@@ -137,3 +137,51 @@ Proof.
   inverts H. simpl. intuition.
 Qed.
 Hint Resolve Forall_map.
+
+
+Lemma Forall_impl_inner
+ :  forall A {B} (P: B -> Prop) xs
+ ,  A
+ -> Forall (fun x => A -> P x) xs
+ -> Forall (fun x => P x) xs.
+Proof.
+ intros.
+ induction xs.
+ - auto.
+ - eapply Forall_cons.
+   + inverts H. auto.
+   + inverts H. auto.
+Qed. 
+
+
+Lemma Forall_insts
+ :  forall {A B} a' xs (P: A -> B -> Prop)
+ ,  Forall (fun x => forall a, P a x) xs
+ -> Forall (fun x => P a' x) xs.
+Proof.
+ intros.
+ induction xs.
+ - auto.
+ - eapply Forall_cons.
+   + inverts H. eapply H2.
+   + inverts H. eapply IHxs. assumption.
+Qed.
+
+
+Lemma Forall_impls
+ :  forall {A} (P Q: A -> Prop) xs
+ ,  Forall (fun x => P x) xs
+ -> Forall (fun x => P x -> Q x) xs
+ -> Forall (fun x => Q x) xs.
+Proof.
+ intros.
+ induction xs.
+ - auto.
+ - eapply Forall_cons.
+   + inverts H. inverts H0.
+     auto.
+   + inverts H. inverts H0. 
+     eapply IHxs. auto. auto.
+Qed.
+
+
